State the Schreier.spec theorem.

B4_group.v
@@ -1,3 +1,40 @@
 (* Basic Group Theory definitions. *)
 
 From CGT Require Import A1_setup B1_fmap B2_perm B3_word.
+Require Import Lia.
+
+Section Group.
+
+Notation can := (prune xH).
+Notation Canonical := (Pruned xH).
+
+(* The generating set of the group. *)
+Variable gen : list perm.
+
+(* Range of the generator after n compositions. *)
+Fixpoint Generates n π :=
+  match n with
+  | O => can π = ident
+  | S m => ∃σ, In σ gen /\ Generates m (σ ∘ π)
+  end.
+
+(* Group membership defined by the generator. *)
+Definition In_Group π := ∃n, Generates n π.
+
+(* Cardinality of the group. *)
+Definition Group_Order (ord : positive) :=
+  ∃f : positive -> perm,
+    (∀i, i <= ord -> Canonical (f i)) /\
+    (∀π, In_Group π -> ∃i, i <= ord /\ f i = can π) /\
+    (∀i j, i <= ord -> j <= ord -> i ≠ j -> f i ≠ f j).
+
+End Group.
+
+Theorem unit_group_order :
+  Group_Order [] 1.
+Proof.
+exists (λ _, ident); repeat split; intros.
+2: lia. destruct H as [[]]; simpl in H.
+exists 1; split; easy.
+destruct H; easy.
+Qed.
